Grounding_Pipeline.thy
@@ -1,9 +1,10 @@
 theory Grounding_Pipeline
   imports Type_Normalization Goal_Normalization Precondition_Normalization
-    PDDL_Relaxation Grounded_PDDL
+    PDDL_Relaxation Pseudo_Datalog Grounded_PDDL PDDL_to_STRIPS
 begin
 
-subsection \<open> Setting up compact notations \<close>
+subsection \<open> Important theorems from individual grounding pipeline steps.
+  Setting up compact notations for some of them to remove contexts. \<close>
 
 context ast_problem begin
 thm detype_prob_sel
@@ -11,14 +12,14 @@ thm ast_problem2.prob_detyped
 lemma detype_prob_wf_compact:
   "restrict_prob \<Longrightarrow> wf_problem
   \<Longrightarrow> ast_problem.wf_problem detype_prob"
-  using restr_problem2.detype_prob_wf
-  using restr_problem2.intro restr_problem.intro restr_problem_axioms.intro wf_ast_problem.intro
+  using restrict_problem2.detype_prob_wf
+  using restrict_problem2.intro restrict_problem.intro restrict_problem_axioms.intro wf_ast_problem.intro
   by auto
 lemma detyped_valid_iff_compact:
   "restrict_prob \<Longrightarrow> wf_problem
   \<Longrightarrow> valid_plan \<pi>s \<longleftrightarrow> ast_problem.valid_plan (detype_prob) \<pi>s"
-  using restr_problem2.detyped_valid_iff
-  using restr_problem2.intro restr_problem.intro restr_problem_axioms.intro wf_ast_problem.intro
+  using restrict_problem2.detyped_valid_iff
+  using restrict_problem2.intro restrict_problem.intro restrict_problem_axioms.intro wf_ast_problem.intro
   by auto
 
 thm ast_problem.degoal_prob_sel
@@ -36,7 +37,7 @@ lemma degoaled_valid_iff_compact:
   using wf_ast_problem3_def wf_ast_problem.intro by simp
 
 thm ast_problem.split_prob_sel
-thm ast_problem4.prec_normed_prob
+thm ast_problem4.prec_normed_dom
 lemma split_prob_wf_compact:
   "wf_problem \<Longrightarrow> ast_problem.wf_problem (split_prob)"
   using wf_ast_problem4.split_prob_wf
@@ -50,32 +51,50 @@ lemma restore_plan_split_valid_compact:
   using wf_ast_problem4.restore_plan_split_valid
   using wf_ast_problem4_def wf_ast_problem.intro by simp
 
-lemma relax_wf_normed_compact:
+lemma relax_wf_relaxed_compact:
   "wf_problem \<Longrightarrow> normalized_prob \<Longrightarrow>
-    ast_problem.normalized_prob relax_prob \<and> ast_problem.wf_problem relax_prob"
-  using normed_prob_rx.relax_normed normed_prob_rx.relax_wf
-  unfolding normed_prob_rx_def normed_prob_def wf_ast_problem_def normed_prob_axioms_def
-  by blast
+    ast_problem.relaxed_prob relax_prob \<and> ast_problem.wf_problem relax_prob"
+  using normalized_problem_rx.relax_relaxes normalized_problem_rx.relax_wf
+  unfolding normalized_problem_rx_def normalized_problem_def' by simp
+lemma relax_normed_compact:
+  "wf_problem \<Longrightarrow> normalized_prob \<Longrightarrow>
+    ast_problem.normalized_prob relax_prob"
+  using normalized_problem_rx.relax_normed
+  unfolding normalized_problem_rx_def normalized_problem_def' by simp
 lemma relax_achievables_compact:
   "wf_problem \<Longrightarrow> normalized_prob \<Longrightarrow>
     {a. achievable a} \<subseteq> {a. ast_problem.achievable relax_prob a}"
-  using normed_prob_rx.relax_achievables
-  unfolding normed_prob_rx_def normed_prob_def wf_ast_problem_def normed_prob_axioms_def
-  by blast
+  using normalized_problem_rx.relax_achievables
+  unfolding normalized_problem_rx_def normalized_problem_def'
+  by simp
 lemma relax_applicables_compact:
   "wf_problem \<Longrightarrow> normalized_prob \<Longrightarrow>
     {\<pi>. applicable \<pi>} \<subseteq> {\<pi>. ast_problem.applicable relax_prob \<pi>}"
-  using normed_prob_rx.relax_applicables
-  unfolding normed_prob_rx_def normed_prob_def wf_ast_problem_def normed_prob_axioms_def
-  by blast
+  using normalized_problem_rx.relax_applicables
+  unfolding normalized_problem_rx_def normalized_problem_def'    
+  by simp
 
-(* lemma needed:
-  wf_problem P \<Longrightarrow> wf_grounder P (relax_reached ops) (relax_reached facts)*)
+(* unproven *)
+thm relaxed_problem.found_facts_achievable
+thm relaxed_problem.found_pactions_applicable
 
 thm grounder.ground_prob_grounded
 thm wf_grounder.ground_prob_wf
+lemma (in wf_grounder) ground_prob_normed:
+  assumes "normalized_prob"
+  shows "ast_problem.normalized_prob ground_prob"
+  sorry
 thm wf_grounder.valid_plan_iff
 thm wf_grounder.valid_plan_left
+
+
+lemma wf_as_strips_compact:
+  "wf_problem \<Longrightarrow> grounded_prob \<Longrightarrow> normalized_prob \<Longrightarrow> is_valid_problem_strips as_strips"
+  using grounded_normalized_problem.wf_as_strips
+  unfolding grounded_normalized_problem_def grounded_normalized_problem_axioms_def
+  unfolding grounded_problem_def grounded_problem_axioms_def wf_ast_problem_def
+  unfolding normalized_prob_def by blast
+  
 
 end
 
@@ -118,9 +137,9 @@ text \<open> Goal normalization only preserves precondition normalization if the
   pure conjunction.\<close>
 
 lemma goal_norm_preserves_prec_norm:
-  assumes "prec_normed_prob"
+  assumes "prec_normed_dom"
     "is_conj (goal P)"
-  shows "ast_problem.prec_normed_prob degoal_prob"
+  shows "ast_domain.prec_normed_dom (domain degoal_prob)"
   using assms(1) unfolding ast_domain.prec_normed_dom_def
   unfolding degoal_prob_sel degoal_dom_sel
   unfolding goal_ac_def term_goal_def
@@ -132,7 +151,8 @@ theorem normalization_normalizes:
   using ast_problem2.prob_detyped
   using ast_problem.degoal_prob_sel(4) ast_problem.goal_norm_preserves_typeless
   using ast_problem.prec_norm_preserves_typeless ast_problem.prec_norm_preserves_goal_conj
-    ast_problem4.prec_normed_prob by simp
+    ast_problem4.prec_normed_dom
+  by (simp add: ast_problem.split_prob_sel(1))
 
 theorem normalization_wf:
   "restrict_prob \<Longrightarrow> wf_problem \<Longrightarrow> ast_problem.wf_problem P\<^sub>N"
@@ -162,15 +182,110 @@ end
 subsection \<open> Relaxation \<close>
 
 context ast_problem begin
-lemma assumes "restrict_prob" "wf_problem"
-  shows "{\<pi>. ast_problem.applicable P\<^sub>N \<pi>} \<subseteq> {\<pi>. ast_problem.applicable (ast_problem.relax_prob P\<^sub>N) \<pi>}"
+
+definition "P\<^sub>R \<equiv> ast_problem.relax_prob P\<^sub>N"
+
+lemma relaxation_applicables:
+  assumes "restrict_prob" "wf_problem"
+  shows "{\<pi>. ast_problem.applicable P\<^sub>N \<pi>} \<subseteq> {\<pi>. ast_problem.applicable P\<^sub>R \<pi>}"
+  unfolding P\<^sub>R_def
   using assms normalization_normalizes normalization_wf ast_problem.relax_applicables_compact by simp
 
-lemma assumes "restrict_prob" "wf_problem"
-  shows "{a. ast_problem.achievable P\<^sub>N a} \<subseteq> {a. ast_problem.achievable (ast_problem.relax_prob P\<^sub>N) a}"
+lemma relaxation_achievables:
+  assumes "restrict_prob" "wf_problem"
+  shows "{a. ast_problem.achievable P\<^sub>N a} \<subseteq> {a. ast_problem.achievable P\<^sub>R a}"
+  unfolding P\<^sub>R_def
   using assms normalization_normalizes normalization_wf ast_problem.relax_achievables_compact by simp
 
+lemma relaxation_wf_relaxed_normed:
+  assumes "restrict_prob" "wf_problem"
+  shows "ast_problem.wf_problem P\<^sub>R" "ast_problem.relaxed_prob P\<^sub>R" "ast_problem.normalized_prob P\<^sub>R"
+  unfolding P\<^sub>R_def
+  using assms normalization_normalizes normalization_wf
+  using ast_problem.relax_wf_relaxed_compact ast_problem.relax_normed_compact
+  by blast+
 
+subsection \<open> Reachability Analysis \<close>
+
+abbreviation "all_facts \<equiv> remdups (snd (ast_problem.semi_naive_eval P\<^sub>R))"
+abbreviation "all_pactions \<equiv> fst (ast_problem.semi_naive_eval P\<^sub>R)"
+
+
+thm relaxed_problem.found_facts_achievable
+
+lemma all_facts_solved:
+  assumes "restrict_prob" "wf_problem"
+  shows "set all_facts = {f. ast_problem.achievable P\<^sub>R f}"
+  using assms relaxed_problem.found_facts_achievable
+  using relaxation_wf_relaxed_normed[OF assms]
+  by (simp add: normalized_problem_def' relaxed_problem.intro relaxed_problem_axioms_def)
+
+lemma wf_grounder_args:
+  assumes "restrict_prob" "wf_problem"
+  shows "wf_grounder P\<^sub>N all_facts all_pactions"
+  unfolding wf_grounder_def apply (intro conjI)
+  using assms normalization_wf apply blast
+          apply simp
+  using relaxation_achievables[OF assms] all_facts_solved[OF assms] apply argo
+  using relaxation_achievables[OF assms] all_facts_solved[OF assms]
+    wf_ast_problem.achievable_wf normalization_wf[OF assms]
+    wf_ast_problem_def
+  apply (metis P\<^sub>R_def assms ast_domain_rx.rx_wf_fmla_atom ast_problem.relax_prob_sel(1) ast_problem_rx.rx_objT mem_Collect_eq relaxation_wf_relaxed_normed(1))
+  sorry
+
+subsection \<open> Grounding \<close>
+
+definition "P\<^sub>G \<equiv> grounder.ground_prob P\<^sub>N all_facts all_pactions"
+definition "reconstruct_plan_ground \<pi>s =
+  reconstruct_plan_norm (grounder.restore_ground_plan all_pactions \<pi>s)"
+
+lemma wf_ground_normed_problem:
+  assumes "restrict_prob" "wf_problem"
+  shows "ast_problem.wf_problem P\<^sub>G" "ast_problem.normalized_prob P\<^sub>G"
+    "ast_problem.grounded_prob P\<^sub>G"
+  using assms wf_grounder_args normalization_normalizes
+  using wf_grounder.ground_prob_wf wf_grounder.ground_prob_normed
+    grounder.ground_prob_grounded
+  by (simp_all add: P\<^sub>G_def)
+
+lemma ground_plan_valid_iff:
+  assumes "restrict_prob" "wf_problem"
+  shows "(\<exists>\<pi>s. valid_plan \<pi>s) \<longleftrightarrow> (\<exists>\<pi>s'. ast_problem.valid_plan P\<^sub>G \<pi>s')"
+  using assms normalization_valid_iff wf_grounder_args
+  using wf_grounder.valid_plan_iff
+  unfolding P\<^sub>G_def by blast
+
+lemma ground_plan_reconstruct:
+  assumes "restrict_prob" "wf_problem"
+  shows "ast_problem.valid_plan P\<^sub>G \<pi>s \<Longrightarrow>
+    valid_plan (reconstruct_plan_ground \<pi>s)"
+  using assms normalization_reconstruct wf_grounder_args
+  using wf_grounder.valid_plan_left normalization_reconstruct
+  unfolding P\<^sub>G_def reconstruct_plan_ground_def by simp
+
+subsection \<open> Conversion to STRIPS \<close>
+definition "P\<^sub>S \<equiv> ast_problem.as_strips P\<^sub>G"
+definition "reconstruct_pipeline_plan ops \<equiv>
+  reconstruct_plan_ground (ast_problem.restore_pddl_plan P\<^sub>G ops)"
+
+lemma wf_as_strips:
+  assumes "restrict_prob" "wf_problem"
+  shows "is_valid_problem_strips P\<^sub>S"
+  using assms ast_problem.wf_as_strips_compact
+  using wf_ground_normed_problem
+  unfolding P\<^sub>S_def by blast
+
+lemma strips_plan_reconstruct:
+  assumes "restrict_prob" "wf_problem"
+  shows "is_serial_solution_for_problem P\<^sub>S ops \<Longrightarrow>
+    valid_plan (reconstruct_pipeline_plan ops)"
+  oops
+
+lemma strips_plan_iff:
+  assumes "restrict_prob" "wf_problem"
+  shows "(\<exists>ops. is_serial_solution_for_problem P\<^sub>S ops) \<longleftrightarrow>
+    (\<exists>\<pi>s. valid_plan \<pi>s)"
+  oops
 
 end
 end
