Normalization_Definitions.thy
@@ -2,14 +2,50 @@ theory Normalization_Definitions
   imports PDDL_Sema_Supplement
 begin
 
-text \<open> The only reason these are here instead of in their respective
+text \<open>This file contains definitions of PDDL normalization properties.
+The only reason these are here instead of in their respective
   normalization files is to reduce dependencies across files.
   This benefits development on my low-RAM laptop.\<close>
+
+(* TODO figure out a way to remove this reduncancy with the locales *)
+lemma "wf_ast_problem p \<longleftrightarrow> ast_problem.wf_problem p"
+  by (simp add: wf_ast_problem_def)
+
+text \<open> Input Restriction \<close>
 
 (* TODO think of a better name *)
 abbreviation "\<omega> \<equiv> Either [''object'']"
 
-(*
+(* This being omitted from wf_action_schema complicates type normalization *)
+definition (in ast_domain) wf_action_params :: "ast_action_schema \<Rightarrow> bool" where
+  "wf_action_params a \<equiv> (\<forall>(n, t) \<in> set (parameters a). wf_type t)"
+
+fun single_type :: "type \<Rightarrow> bool" where
+  "single_type (Either ts) \<longleftrightarrow> length ts = 1"
+abbreviation single_types :: "('a \<times> type) list \<Rightarrow> bool" where
+  "single_types os \<equiv> \<forall>(_, T) \<in> set os. single_type T"
+
+definition (in ast_domain) restrict_dom :: bool where
+  "restrict_dom \<equiv> single_types (consts D)
+                  \<and> list_all1 wf_action_params (actions D)"
+
+locale restrict_domain = wf_ast_domain +
+  assumes restrict_dom: restrict_dom
+lemmas restrict_domain_def' =
+  restrict_domain_def[unfolded wf_ast_domain_def restrict_domain_axioms_def]
+
+definition (in ast_problem) "restrict_prob \<equiv> restrict_dom \<and> single_types (objects P)"
+
+locale restrict_problem = wf_ast_problem +
+  assumes restrict_prob: restrict_prob
+lemmas restrict_problem_def' =
+  restrict_problem_def[unfolded wf_ast_problem_def restrict_problem_axioms_def]
+
+sublocale restrict_problem \<subseteq> restrict_domain "D"
+  using restrict_prob restrict_prob_def by (unfold_locales) simp
+
+
+text \<open> Type normalization:
 - type hierarchy is empty (implicitly includes ''object'')
 - Everything else is Either [''object''].
   This is a little superfluous: If well-formed, they can only be [''object'', ''object'', ...],
@@ -17,63 +53,105 @@ abbreviation "\<omega> \<equiv> Either [''object'']"
   - predicate argument types are Either [''object''].
   - const types are Either [''object'']
   - actions parameters are detyped
-    This isn't superfluous because wf_action_schema does not ensure well-formed param types. *)
-definition (in ast_domain) typeless_dom :: "bool" where
-  "typeless_dom \<equiv>
+    This isn't superfluous because wf_action_schema does not ensure well-formed param types. \<close>
+definition (in ast_domain) "typeless_dom \<equiv>
     types D = []
     \<and> (\<forall>p \<in> set (predicates D). \<forall>T \<in> set (argTs p). T = \<omega>)
     \<and> (\<forall>(n, T) \<in> set (consts D). T = \<omega>)
     \<and> (\<forall>ac \<in> set (actions D). \<forall>(n, T) \<in> set (ac_params ac). T = \<omega>)"
 
-(*
+(*locale typeless_domain = wf_ast_domain +
+  assumes typeless_dom: typeless_dom
+lemmas typeless_domain_def' =
+  typeless_domain_def[unfolded wf_ast_domain_def typeless_domain_axioms_def]*)
+
+text \<open>
 - domain is detyped
-- objects are detyped
-*)
-definition (in ast_problem) typeless_prob :: "bool" where
-  "typeless_prob \<equiv>
-    typeless_dom
-    \<and> (\<forall>(n, T) \<in> set (objects P). T = \<omega>)"
+- objects are detyped \<close>
+definition (in ast_problem) "typeless_prob \<equiv>
+  typeless_dom \<and> (\<forall>(n, T) \<in> set (objects P). T = \<omega>)"
 
-definition (in ast_domain) "prec_normed_dom \<equiv>
-  \<forall>ac \<in> set (actions D). is_conj (ac_pre ac)"
+(*locale typeless_problem = wf_ast_problem +
+  assumes typeless_prob: typeless_prob
+lemmas typeless_problem_def' =
+  typeless_problem_def[unfolded wf_ast_problem_def typeless_problem_axioms_def]
 
-abbreviation (in ast_problem) (input) "prec_normed_prob \<equiv> prec_normed_dom"
+sublocale typeless_problem \<subseteq> typeless_domain D
+  using typeless_prob typeless_prob_def by (unfold_locales) blast *)
 
-definition (in ast_domain) "normalized_dom \<equiv>
-  typeless_dom \<and> prec_normed_dom"
+text \<open> Precondition normalization: all action preconditions are normalized. \<close>
+
+definition (in ast_domain) "prec_normed_dom \<equiv> \<forall>ac \<in> set (actions D). is_conj (ac_pre ac)"
+
+(*locale precond_normed_domain = wf_ast_domain +
+  assumes prec_normed_dom: prec_normed_dom
+lemmas precond_normed_domain_def' =
+  precond_normed_domain_def[unfolded wf_ast_domain_def precond_normed_domain_axioms_def]*)
+
+text \<open> Preconditions only exist in the domain, so no additional definition is needed for the problem.\<close>
+
+(*locale precond_normed_problem = wf_ast_problem +
+  assumes prec_normed_prob: prec_normed_dom
+lemmas precond_normed_problem_def' =
+  precond_normed_problem_def[unfolded wf_ast_problem_def precond_normed_problem_axioms_def]
+
+sublocale precond_normed_problem \<subseteq> precond_normed_domain D
+  using prec_normed_prob by (unfold_locales) simp*)
+
+text \<open> Complete normalization additionally assumes that the goal is a conjunction. \<close>
+
+definition (in ast_domain) "normalized_dom \<equiv> typeless_dom \<and> prec_normed_dom"
+
+locale normalized_domain = wf_ast_domain +
+  assumes normalized_dom: normalized_dom
+lemmas normalized_domain_def' =
+  normalized_domain_def[unfolded wf_ast_domain_def normalized_domain_axioms_def]
+
+(*sublocale normalized_domain \<subseteq> typeless_domain D
+  using normalized_dom normalized_dom_def by (unfold_locales) simp
+
+sublocale normalized_domain \<subseteq> precond_normed_domain D
+  using normalized_dom normalized_dom_def by (unfold_locales) simp*)
 
 definition (in ast_problem) "normalized_prob \<equiv>
-  typeless_prob \<and> (is_conj (goal P)) \<and> prec_normed_prob"
+  typeless_prob \<and> prec_normed_dom \<and> is_conj (goal P)"
 
-lemma (in ast_problem) normed_prob_normed_dom:
-  "normalized_prob \<Longrightarrow> normalized_dom"
-  unfolding normalized_prob_def normalized_dom_def typeless_prob_def by blast
+locale normalized_problem = wf_ast_problem +
+  assumes normalized_prob: normalized_prob
+lemmas normalized_problem_def' =
+  normalized_problem_def[unfolded wf_ast_problem_def normalized_problem_axioms_def]
+
+sublocale normalized_problem \<subseteq> normalized_domain D
+  using normalized_prob normalized_dom_def normalized_prob_def typeless_prob_def
+  by (unfold_locales) blast
+
+(*sublocale normalized_problem \<subseteq> typeless_problem P
+  using normalized_prob normalized_prob_def by (unfold_locales) simp
+
+sublocale normalized_problem \<subseteq> precond_normed_problem P
+  using normalized_prob normalized_prob_def by (unfold_locales) simp*)
+
+text \<open> Relaxation \<close>
 
 definition (in ast_domain) "relaxed_dom \<equiv>
   normalized_dom \<and> (\<forall>a \<in> set (actions D). is_pos_conj (ac_pre a))"
 
-definition (in ast_problem) "relaxed_prob \<equiv>
-  normalized_prob \<and> is_pos_conj (goal P) \<and>
-    (\<forall>a \<in> set (actions D). is_pos_conj (ac_pre a))"
+locale relaxed_domain = normalized_domain +
+  assumes relaxed_dom: relaxed_dom
 
-(* contexts *)
+definition (in ast_problem) "relaxed_prob \<equiv> normalized_prob \<and>
+  is_pos_conj (goal P) \<and> (\<forall>a \<in> set (actions D). is_pos_conj (ac_pre a))"
 
-term wf_ast_problem
+locale relaxed_problem = normalized_problem +
+  assumes relaxed_prob: relaxed_prob
 
-locale normed_dom = wf_ast_domain D for D +
-  assumes normed_dom: normalized_dom
+sublocale relaxed_problem \<subseteq> relaxed_domain D
+  using relaxed_prob normalized_dom relaxed_prob_def relaxed_dom_def
+  by (unfold_locales) simp
 
-locale normed_prob = wf_ast_problem P for P +
-  assumes normed_prob: normalized_prob
-
-sublocale normed_prob \<subseteq> normed_dom D
-  apply (unfold_locales)
-  using normed_prob normed_prob_normed_dom by simp
-
-locale wf_relaxed_normed_prob = wf_ast_problem +
-  assumes relaxed: relaxed_prob and normed: normalized_prob
-
-(* reachability definitions *)
+subsection \<open> Reachability Definitions \<close>
+text \<open> A plan action is applicable if there exists some plan that executes it.
+  Whether or not this plan actually solves the task doesn't matter.\<close>
 
 definition (in ast_problem) applicable :: "plan_action \<Rightarrow> bool"
   where "applicable \<pi> \<equiv> \<exists>\<pi>s M. plan_action_path I \<pi>s M \<and> \<pi> \<in> set \<pi>s"
@@ -101,6 +179,8 @@ next
   ultimately show "applicable \<pi>" using 1 applicable_def plan_action_path_append_intro by fast
 qed
 
+text \<open> A fact is achievable if there exists some plan that results in a state containing it. \<close>
+
 definition (in ast_problem) achievable :: "object atom formula \<Rightarrow> bool"
   where "achievable a \<equiv> \<exists>\<pi>s M. plan_action_path I \<pi>s M \<and> a \<in> M"
 
@@ -111,13 +191,17 @@ proof -
   thus ?thesis unfolding achievable_def I_def by blast
 qed
 
+lemma (in wf_ast_problem) achievable_wf:
+  "achievable a \<Longrightarrow> wf_fmla_atom objT a"
+  unfolding achievable_def
+  using wf_I wf_plan_action_path
+  unfolding wf_world_model_def by meson
+
 lemma (in wf_ast_problem) achievable_predAtm:
   "achievable a \<Longrightarrow> is_predAtom a"
-  unfolding achievable_def
-  using wf_I wf_plan_action_path wf_world_model_def
-  unfolding wf_fmla_atom_alt by meson
+  using achievable_wf wf_fmla_atom_alt by blast
 
-(* grounded PDDL *)
+subsection \<open> Grounded PDDL \<close>
 
 text \<open>
   Types, constants and objects don't really matter for grounded PDDL: they can just be ignored.
@@ -136,21 +220,19 @@ definition (in ast_domain) "grounded_dom \<equiv>
   consts D = [] \<and>
   list_all1 grounded_ac (actions D)"
 
-definition (in ast_problem) "grounded_prob \<equiv>
-  grounded_dom \<and>
-  objects P = []"
-
-
-locale wf_grounded_domain = wf_ast_domain +
+locale grounded_domain = wf_ast_domain +
   assumes grounded_dom: grounded_dom
 
-locale wf_grounded_problem = wf_ast_problem +
+definition (in ast_problem) "grounded_prob \<equiv>
+  grounded_dom \<and> objects P = []"
+
+locale grounded_problem = wf_ast_problem +
   assumes grounded_prob: grounded_prob
 
-sublocale wf_grounded_problem \<subseteq> wf_grounded_domain D
+sublocale grounded_problem \<subseteq> grounded_domain D
   using grounded_prob grounded_prob_def by (unfold_locales) simp
 
-lemma (in wf_grounded_problem) grounded_pa_nullary:
+lemma (in grounded_problem) grounded_pa_nullary:
   "wf_plan_action (PAction n args) \<longleftrightarrow> n \<in> ac_name ` set (actions D) \<and> args = []" (is "?L \<longleftrightarrow> ?R")
 proof -
   have empty: "ac_params ac = []" if "ac \<in> set (actions D)" for ac
@@ -170,15 +252,16 @@ proof -
   qed
 qed
 
-(* grounded, normalized PDDL *)
+text \<open> Grounded and normalized PDDL, which is convertible to STRIPS \<close>
 
-locale wf_normed_grounded_domain = wf_grounded_domain +
+(* type normalization follows from grounded domain *)
+locale grounded_normalized_domain = grounded_domain +
   assumes normed_dom: prec_normed_dom
 
-locale wf_normed_grounded_problem = wf_grounded_problem +
-  assumes normed_prob: "prec_normed_prob \<and> (is_conj (goal P))"
+locale grounded_normalized_problem = grounded_problem +
+  assumes normed_prob: "prec_normed_dom \<and> (is_conj (goal P))"
 
-sublocale wf_normed_grounded_problem \<subseteq> wf_normed_grounded_domain D
+sublocale grounded_normalized_problem \<subseteq> grounded_normalized_domain D
   using normed_prob by (unfold_locales) blast
 
 
