Datalog_Utils.thy
@@ -1,8 +1,0 @@
-theory Datalog_Utils
-  imports "../LTS-formalization/Datalog/Datalog"
-begin
-
-
-
-
-end
